@prefix : <https://w3id.org/sirius/ontology/hero/> .
@prefix owl: <http://www.w3.org/2002/07/owl#> .
@prefix rdf: <http://www.w3.org/1999/02/22-rdf-syntax-ns#> .
@prefix xml: <http://www.w3.org/XML/1998/namespace> .
@prefix xsd: <http://www.w3.org/2001/XMLSchema#> .
@prefix rdfs: <http://www.w3.org/2000/01/rdf-schema#> .
@base <https://w3id.org/sirius/ontology/hero/> .

<https://w3id.org/sirius/ontology/hero/> rdf:type owl:Ontology ;
                                          owl:versionIRI <https://w3id.org/sirius/ontology/hero/1.0.0/> ;
                                          owl:imports <http://www.ontologydesignpatterns.org/cp/owl/classification.owl> ,
                                                      <http://www.ontologydesignpatterns.org/cp/owl/observation.owl> ,
                                                      <http://www.ontologydesignpatterns.org/cp/owl/participation.owl> ,
                                                      <http://www.ontologydesignpatterns.org/cp/owl/region.owl> ,
                                                      <http://www.ontologydesignpatterns.org/cp/owl/timeindexedsituation.owl> ,
                                                      <http://www.ontologydesignpatterns.org/cp/owl/timeinterval.owl> ;
                                          <http://purl.org/dc/elements/1.1/creator> "Barzaghi, Sebastian" ;
                                          <http://purl.org/dc/elements/1.1/date> "2023-11-30"^^xsd:date ;
                                          <http://purl.org/dc/terms/abstract> "The Heritage Risk Assessment Ontology (HeRO, https://w3id.org/sirius/ontology/hero) is an OWL 2 DL ontology that aims to provide a framework for the formal description of risk assessment activities related to heritage."@en ;
                                          <http://purl.org/dc/terms/bibliographicCitation> "Barzaghi, S. (2023). Heritage Risk Assessment Ontology. https://w3id.org/sirius/ontology/hero."@en ;
                                          <http://purl.org/dc/terms/created> "2023-11-30"^^xsd:date ;
                                          <http://purl.org/dc/terms/issued> "2023-11-30"^^xsd:date ;
                                          <http://purl.org/dc/terms/license> "http://creativecommons.org/licenses/by/4.0/"@en ;
                                          <http://purl.org/dc/terms/publisher> "Barzaghi, Sebastian"@en ;
                                          <http://purl.org/dc/terms/source> """
        https://doi.org/10.6084/M9.FIGSHARE.3189769.V2
        """@en ,
                                                                            """
        https://www.canada.ca/en/conservation-institute/services/risk-management-heritage-collections/abc-method-risk-management-approach.html
        """@en ,
                                                                            """
        https://www.iccrom.org/sites/default/files/2017-12/risk_manual_2016-eng.pdf
        """@en ;
                                          <http://purl.org/dc/terms/title> "Heritage Risk Assessment Ontology (HeRO)"@en ;
                                          <http://purl.org/vocab/vann/preferredNamespacePrefix> "hero"@en ;
                                          <http://purl.org/vocab/vann/preferredNamespaceUri> "https://w3id.org/sirius/ontology/hero/"@en ;
                                          rdfs:comment "The Heritage Risk Assessment Ontology (HeRO, https://w3id.org/sirius/ontology/hero) is an OWL 2 DL ontology that aims to provide a framework for the formal description of risk assessment activities related to heritage."@en ;
                                          owl:versionInfo "1.0.0" ;
                                          <http://www.w3.org/2003/06/sw-vocab-status/ns#status> "work in progress"@en .

#################################################################
#    Annotation properties
#################################################################

###  http://purl.org/dc/elements/1.1/creator
<http://purl.org/dc/elements/1.1/creator> rdf:type owl:AnnotationProperty .


###  http://purl.org/dc/elements/1.1/date
<http://purl.org/dc/elements/1.1/date> rdf:type owl:AnnotationProperty .


###  http://purl.org/dc/elements/1.1/description
<http://purl.org/dc/elements/1.1/description> rdf:type owl:AnnotationProperty .


###  http://purl.org/dc/elements/1.1/title
<http://purl.org/dc/elements/1.1/title> rdf:type owl:AnnotationProperty .


###  http://purl.org/dc/terms/abstract
<http://purl.org/dc/terms/abstract> rdf:type owl:AnnotationProperty .


###  http://purl.org/dc/terms/bibliographicCitation
<http://purl.org/dc/terms/bibliographicCitation> rdf:type owl:AnnotationProperty .


###  http://purl.org/dc/terms/created
<http://purl.org/dc/terms/created> rdf:type owl:AnnotationProperty .


###  http://purl.org/dc/terms/issued
<http://purl.org/dc/terms/issued> rdf:type owl:AnnotationProperty .


###  http://purl.org/dc/terms/license
<http://purl.org/dc/terms/license> rdf:type owl:AnnotationProperty .


###  http://purl.org/dc/terms/publisher
<http://purl.org/dc/terms/publisher> rdf:type owl:AnnotationProperty .


###  http://purl.org/dc/terms/source
<http://purl.org/dc/terms/source> rdf:type owl:AnnotationProperty .


###  http://purl.org/dc/terms/title
<http://purl.org/dc/terms/title> rdf:type owl:AnnotationProperty .


###  http://purl.org/vocab/vann/preferredNamespacePrefix
<http://purl.org/vocab/vann/preferredNamespacePrefix> rdf:type owl:AnnotationProperty .


###  http://purl.org/vocab/vann/preferredNamespaceUri
<http://purl.org/vocab/vann/preferredNamespaceUri> rdf:type owl:AnnotationProperty .


###  http://www.ontologydesignpatterns.org/schemas/cpannotationschema.owl#coversRequirements
<http://www.ontologydesignpatterns.org/schemas/cpannotationschema.owl#coversRequirements> rdf:type owl:AnnotationProperty .


###  http://www.ontologydesignpatterns.org/schemas/cpannotationschema.owl#extractedFrom
<http://www.ontologydesignpatterns.org/schemas/cpannotationschema.owl#extractedFrom> rdf:type owl:AnnotationProperty .


###  http://www.ontologydesignpatterns.org/schemas/cpannotationschema.owl#hasAuthor
<http://www.ontologydesignpatterns.org/schemas/cpannotationschema.owl#hasAuthor> rdf:type owl:AnnotationProperty .


###  http://www.ontologydesignpatterns.org/schemas/cpannotationschema.owl#hasComponent
<http://www.ontologydesignpatterns.org/schemas/cpannotationschema.owl#hasComponent> rdf:type owl:AnnotationProperty .


###  http://www.ontologydesignpatterns.org/schemas/cpannotationschema.owl#hasConsequences
<http://www.ontologydesignpatterns.org/schemas/cpannotationschema.owl#hasConsequences> rdf:type owl:AnnotationProperty .


###  http://www.ontologydesignpatterns.org/schemas/cpannotationschema.owl#hasIntent
<http://www.ontologydesignpatterns.org/schemas/cpannotationschema.owl#hasIntent> rdf:type owl:AnnotationProperty .


###  http://www.ontologydesignpatterns.org/schemas/cpannotationschema.owl#hasUnitTest
<http://www.ontologydesignpatterns.org/schemas/cpannotationschema.owl#hasUnitTest> rdf:type owl:AnnotationProperty .


###  http://www.ontologydesignpatterns.org/schemas/cpannotationschema.owl#isSpecializationOf
<http://www.ontologydesignpatterns.org/schemas/cpannotationschema.owl#isSpecializationOf> rdf:type owl:AnnotationProperty .


###  http://www.ontologydesignpatterns.org/schemas/cpannotationschema.owl#relatedCPs
<http://www.ontologydesignpatterns.org/schemas/cpannotationschema.owl#relatedCPs> rdf:type owl:AnnotationProperty .


###  http://www.ontologydesignpatterns.org/schemas/cpannotationschema.owl#scenarios
<http://www.ontologydesignpatterns.org/schemas/cpannotationschema.owl#scenarios> rdf:type owl:AnnotationProperty .


###  http://www.w3.org/2000/01/rdf-schema#comment
rdfs:comment rdf:type owl:AnnotationProperty .


###  http://www.w3.org/2000/01/rdf-schema#isDefinedBy
rdfs:isDefinedBy rdf:type owl:AnnotationProperty .


###  http://www.w3.org/2000/01/rdf-schema#label
rdfs:label rdf:type owl:AnnotationProperty .


###  http://www.w3.org/2001/XMLSchema#citation
xsd:citation rdf:type owl:AnnotationProperty .


###  http://www.w3.org/2002/07/owl#versionInfo
owl:versionInfo rdf:type owl:AnnotationProperty .


###  http://www.w3.org/2003/06/sw-vocab-status/ns#status
<http://www.w3.org/2003/06/sw-vocab-status/ns#status> rdf:type owl:AnnotationProperty .


#################################################################
#    Datatypes
#################################################################

###  http://www.w3.org/2001/XMLSchema#date
xsd:date rdf:type rdfs:Datatype .


#################################################################
#    Object Properties
#################################################################

###  http://www.ontologydesignpatterns.org/cp/owl/classification.owl#classifies
<http://www.ontologydesignpatterns.org/cp/owl/classification.owl#classifies> rdf:type owl:ObjectProperty ;
                                                                             owl:inverseOf <http://www.ontologydesignpatterns.org/cp/owl/classification.owl#isClassifiedBy> ;
                                                                             rdfs:domain <http://www.ontologydesignpatterns.org/cp/owl/classification.owl#Concept> ;
                                                                             rdfs:range owl:Thing ;
                                                                             rdfs:comment "A relation between a Concept and an Entity, e.g. the Role 'student' classifies a Person 'John'." ;
                                                                             rdfs:isDefinedBy <http://www.ontologydesignpatterns.org/cp/owl/classification.owl> ;
                                                                             rdfs:label "classifica"@it ,
                                                                                        "classifies"@en .


###  http://www.ontologydesignpatterns.org/cp/owl/classification.owl#isClassifiedBy
<http://www.ontologydesignpatterns.org/cp/owl/classification.owl#isClassifiedBy> rdf:type owl:ObjectProperty ;
                                                                                 rdfs:domain owl:Thing ;
                                                                                 rdfs:range <http://www.ontologydesignpatterns.org/cp/owl/classification.owl#Concept> ;
                                                                                 rdfs:comment "A relation between a Concept and an Entity, e.g. 'John is considered a typical rude man'; your last concert constitutes the achievement of a lifetime; '20-year-old means she's mature enough'." ;
                                                                                 rdfs:isDefinedBy <http://www.ontologydesignpatterns.org/cp/owl/classification.owl> ;
                                                                                 rdfs:label "is classified by"@en ,
                                                                                            "è classificato da"@it .


###  http://www.ontologydesignpatterns.org/cp/owl/observation.owl#hasObservation
<http://www.ontologydesignpatterns.org/cp/owl/observation.owl#hasObservation> rdf:type owl:ObjectProperty ;
                                                                              rdfs:subPropertyOf <http://www.ontologydesignpatterns.org/cp/owl/situation.owl#hasSetting> ;
                                                                              owl:inverseOf <http://www.ontologydesignpatterns.org/cp/owl/observation.owl#isObservationOf> ;
                                                                              rdfs:domain owl:Thing ;
                                                                              rdfs:range <http://www.ontologydesignpatterns.org/cp/owl/observation.owl#Observation> ;
                                                                              rdfs:comment "The relationship between an entity and an Observation."@en ;
                                                                              rdfs:isDefinedBy <http://www.ontologydesignpatterns.org/cp/owl/observation.owl> ;
                                                                              rdfs:label "has observation"@en .


###  http://www.ontologydesignpatterns.org/cp/owl/observation.owl#hasParameter
<http://www.ontologydesignpatterns.org/cp/owl/observation.owl#hasParameter> rdf:type owl:ObjectProperty ;
                                                                            rdfs:subPropertyOf <http://www.ontologydesignpatterns.org/cp/owl/situation.owl#isSettingFor> ;
                                                                            owl:inverseOf <http://www.ontologydesignpatterns.org/cp/owl/observation.owl#isParameterOf> ;
                                                                            rdfs:domain <http://www.ontologydesignpatterns.org/cp/owl/observation.owl#Observation> ;
                                                                            rdfs:range <http://www.ontologydesignpatterns.org/cp/owl/observation.owl#Parameter> ;
                                                                            rdfs:comment "The relationship between an Observation and a Parameter."@en ;
                                                                            rdfs:isDefinedBy <http://www.ontologydesignpatterns.org/cp/owl/observation.owl> ;
                                                                            rdfs:label "has parameter"@en .


###  http://www.ontologydesignpatterns.org/cp/owl/observation.owl#isObservationOf
<http://www.ontologydesignpatterns.org/cp/owl/observation.owl#isObservationOf> rdf:type owl:ObjectProperty ;
                                                                               rdfs:subPropertyOf <http://www.ontologydesignpatterns.org/cp/owl/situation.owl#isSettingFor> ;
                                                                               rdfs:domain <http://www.ontologydesignpatterns.org/cp/owl/observation.owl#Observation> ;
                                                                               rdfs:range owl:Thing ;
                                                                               rdfs:comment "The relationship between an Observation and an entity it observes."@en ;
                                                                               rdfs:isDefinedBy <http://www.ontologydesignpatterns.org/cp/owl/observation.owl> ;
                                                                               rdfs:label "is observation of"@en .


###  http://www.ontologydesignpatterns.org/cp/owl/observation.owl#isParameterOf
<http://www.ontologydesignpatterns.org/cp/owl/observation.owl#isParameterOf> rdf:type owl:ObjectProperty ;
                                                                             rdfs:subPropertyOf <http://www.ontologydesignpatterns.org/cp/owl/situation.owl#hasSetting> ;
                                                                             rdfs:domain <http://www.ontologydesignpatterns.org/cp/owl/observation.owl#Parameter> ;
                                                                             rdfs:range <http://www.ontologydesignpatterns.org/cp/owl/observation.owl#Observation> ;
                                                                             rdfs:comment "The relationship between a Parameter and an Observation."@en ;
                                                                             rdfs:isDefinedBy <http://www.ontologydesignpatterns.org/cp/owl/observation.owl> ;
                                                                             rdfs:label "is parameter of"@en .


###  http://www.ontologydesignpatterns.org/cp/owl/participation.owl#hasParticipant
<http://www.ontologydesignpatterns.org/cp/owl/participation.owl#hasParticipant> rdf:type owl:ObjectProperty ;
                                                                                owl:inverseOf <http://www.ontologydesignpatterns.org/cp/owl/participation.owl#isParticipantIn> ;
                                                                                rdfs:domain <http://www.ontologydesignpatterns.org/cp/owl/participation.owl#Event> ;
                                                                                rdfs:range <http://www.ontologydesignpatterns.org/cp/owl/participation.owl#Object> ;
                                                                                rdfs:comment "The relationship between a Event and a Object participating in it."@en ;
                                                                                rdfs:isDefinedBy <http://www.ontologydesignpatterns.org/cp/owl/participation.owl> ;
                                                                                rdfs:label "has participant"@en .


###  http://www.ontologydesignpatterns.org/cp/owl/participation.owl#isParticipantIn
<http://www.ontologydesignpatterns.org/cp/owl/participation.owl#isParticipantIn> rdf:type owl:ObjectProperty ;
                                                                                 rdfs:domain <http://www.ontologydesignpatterns.org/cp/owl/participation.owl#Object> ;
                                                                                 rdfs:range <http://www.ontologydesignpatterns.org/cp/owl/participation.owl#Event> ;
                                                                                 rdfs:comment "The relationship between an Object and an Event it participates in."@en ;
                                                                                 rdfs:isDefinedBy <http://www.ontologydesignpatterns.org/cp/owl/participation.owl> ;
                                                                                 rdfs:label "is participant in"@en .


###  http://www.ontologydesignpatterns.org/cp/owl/region.owl#hasRegion
<http://www.ontologydesignpatterns.org/cp/owl/region.owl#hasRegion> rdf:type owl:ObjectProperty ;
                                                                    owl:inverseOf <http://www.ontologydesignpatterns.org/cp/owl/region.owl#isRegionFor> ;
                                                                    rdfs:domain owl:Thing ;
                                                                    rdfs:range <http://www.ontologydesignpatterns.org/cp/owl/region.owl#Region> ;
                                                                    rdfs:comment "A relation between entities and regions, e.g. 'the number of wheels of that truck is 12'." ;
                                                                    rdfs:isDefinedBy <http://www.ontologydesignpatterns.org/cp/owl/region.owl> ;
                                                                    rdfs:label "ha regione"@it ,
                                                                               "has region"@en .


###  http://www.ontologydesignpatterns.org/cp/owl/region.owl#isRegionFor
<http://www.ontologydesignpatterns.org/cp/owl/region.owl#isRegionFor> rdf:type owl:ObjectProperty ;
                                                                      rdfs:domain <http://www.ontologydesignpatterns.org/cp/owl/region.owl#Region> ;
                                                                      rdfs:range owl:Thing ;
                                                                      rdfs:comment "A relation between entities and regions, e.g. 'the color of my car is red'." ;
                                                                      rdfs:isDefinedBy <http://www.ontologydesignpatterns.org/cp/owl/region.owl> ;
                                                                      rdfs:label "is region for"@en ,
                                                                                 "è un ragione di"@it .


###  http://www.ontologydesignpatterns.org/cp/owl/situation.owl#hasSetting
<http://www.ontologydesignpatterns.org/cp/owl/situation.owl#hasSetting> rdf:type owl:ObjectProperty .


###  http://www.ontologydesignpatterns.org/cp/owl/situation.owl#isSettingFor
<http://www.ontologydesignpatterns.org/cp/owl/situation.owl#isSettingFor> rdf:type owl:ObjectProperty ;
                                                                          rdfs:comment "The relationship between a Situation and something it is the setting for."@en .


###  http://www.ontologydesignpatterns.org/cp/owl/timeindexedsituation.owl#atTime
<http://www.ontologydesignpatterns.org/cp/owl/timeindexedsituation.owl#atTime> rdf:type owl:ObjectProperty ;
                                                                               rdfs:subPropertyOf <http://www.ontologydesignpatterns.org/cp/owl/situation.owl#isSettingFor> ;
                                                                               owl:inverseOf <http://www.ontologydesignpatterns.org/cp/owl/timeindexedsituation.owl#isTimeIndexFor> ;
                                                                               rdfs:domain <http://www.ontologydesignpatterns.org/cp/owl/timeindexedsituation.owl#TimeIndexedSituation> ;
                                                                               rdfs:range <http://www.ontologydesignpatterns.org/cp/owl/timeinterval.owl#TimeInterval> ;
                                                                               rdfs:comment "The relationship between a Time indexed situation and a Time interval."@en ;
                                                                               rdfs:isDefinedBy <http://www.ontologydesignpatterns.org/cp/owl/timeindexedsituation.owl> ;
                                                                               rdfs:label "at time"@en .


###  http://www.ontologydesignpatterns.org/cp/owl/timeindexedsituation.owl#forEntity
<http://www.ontologydesignpatterns.org/cp/owl/timeindexedsituation.owl#forEntity> rdf:type owl:ObjectProperty ;
                                                                                  rdfs:subPropertyOf <http://www.ontologydesignpatterns.org/cp/owl/situation.owl#isSettingFor> ;
                                                                                  owl:inverseOf <http://www.ontologydesignpatterns.org/cp/owl/timeindexedsituation.owl#hasTimeIndexedSetting> ;
                                                                                  rdfs:domain <http://www.ontologydesignpatterns.org/cp/owl/timeindexedsituation.owl#TimeIndexedSituation> ;
                                                                                  rdfs:range owl:Thing ;
                                                                                  rdfs:comment "The relationship between a Time indexed situation and something contextualised in it."@en ;
                                                                                  rdfs:isDefinedBy <http://www.ontologydesignpatterns.org/cp/owl/timeindexedsituation.owl> ;
                                                                                  rdfs:label "for entity"@en .


###  http://www.ontologydesignpatterns.org/cp/owl/timeindexedsituation.owl#hasTimeIndexedSetting
<http://www.ontologydesignpatterns.org/cp/owl/timeindexedsituation.owl#hasTimeIndexedSetting> rdf:type owl:ObjectProperty ;
                                                                                              rdfs:subPropertyOf <http://www.ontologydesignpatterns.org/cp/owl/situation.owl#hasSetting> ;
                                                                                              rdfs:domain owl:Thing ;
                                                                                              rdfs:range <http://www.ontologydesignpatterns.org/cp/owl/timeindexedsituation.owl#TimeIndexedSituation> ;
                                                                                              rdfs:comment "The relationship between an entity and a Time indexed situation contextualising it."@en ;
                                                                                              rdfs:isDefinedBy <http://www.ontologydesignpatterns.org/cp/owl/timeindexedsituation.owl> ;
                                                                                              rdfs:label "has time indexed setting"@en .


###  http://www.ontologydesignpatterns.org/cp/owl/timeindexedsituation.owl#isTimeIndexFor
<http://www.ontologydesignpatterns.org/cp/owl/timeindexedsituation.owl#isTimeIndexFor> rdf:type owl:ObjectProperty ;
                                                                                       rdfs:subPropertyOf <http://www.ontologydesignpatterns.org/cp/owl/situation.owl#hasSetting> ;
                                                                                       rdfs:domain <http://www.ontologydesignpatterns.org/cp/owl/timeinterval.owl#TimeInterval> ;
                                                                                       rdfs:range <http://www.ontologydesignpatterns.org/cp/owl/timeindexedsituation.owl#TimeIndexedSituation> ;
                                                                                       rdfs:comment "The relationship between a Time interval and a Time indexed situation."@en ;
                                                                                       rdfs:isDefinedBy <http://www.ontologydesignpatterns.org/cp/owl/timeindexedsituation.owl> ;
                                                                                       rdfs:label "is time index for"@en .


###  https://w3id.org/sirius/ontology/hero/analyses
:analyses rdf:type owl:ObjectProperty ;
          rdfs:subPropertyOf :assesses ;
          owl:inverseOf :isAnalysedIn ;
          rdfs:domain :AnalysisDescription ;
          rdfs:range :Risk ;
          rdfs:comment "The relationship between an analysis and a risk that is being analysed."@en ;
          rdfs:isDefinedBy <https://w3id.org/sirius/ontology/hero> ;
          rdfs:label "analyses"@en .


###  https://w3id.org/sirius/ontology/hero/assesses
:assesses rdf:type owl:ObjectProperty ;
          rdfs:subPropertyOf <http://www.ontologydesignpatterns.org/cp/owl/timeindexedsituation.owl#forEntity> ;
          owl:inverseOf :isAssessedIn ;
          rdfs:domain :AssessmentActivity ;
          rdfs:range :Element ;
          rdfs:comment "A relationship between an assessment activity and an entity assessed by it, such as a criterion."@en ;
          rdfs:isDefinedBy <https://w3id.org/sirius/ontology/hero> ;
          rdfs:label "assesses"@en .


###  https://w3id.org/sirius/ontology/hero/assigns
:assigns rdf:type owl:ObjectProperty ;
         rdfs:subPropertyOf :assesses ;
         owl:inverseOf :isAssignedIn ;
         rdfs:domain :ValueDescription ;
         rdfs:range :Value ;
         rdfs:comment "The relationship between a value assessment and an asset value that is being assessed."@en ;
         rdfs:isDefinedBy <https://w3id.org/sirius/ontology/hero> ;
         rdfs:label "assigns"@en .


###  https://w3id.org/sirius/ontology/hero/describes
:describes rdf:type owl:ObjectProperty ;
           rdfs:subPropertyOf <http://www.ontologydesignpatterns.org/cp/owl/participation.owl#hasParticipant> ,
                              <http://www.ontologydesignpatterns.org/cp/owl/situation.owl#isSettingFor> ;
           owl:inverseOf :isDescribedIn ;
           rdfs:domain :AssessmentActivity ;
           rdfs:range owl:Thing ;
           rdfs:comment "The relationship between an assessment activity and the entity described in that assessment, such as an asset."@en ;
           rdfs:isDefinedBy <https://w3id.org/sirius/ontology/hero> ;
           rdfs:label "describes"@en .


###  https://w3id.org/sirius/ontology/hero/documents
:documents rdf:type owl:ObjectProperty ;
           owl:inverseOf :isDocumentedBy ;
           rdfs:domain <http://xmlns.com/foaf/0.1/Document> ;
           rdfs:range owl:Thing ;
           rdfs:comment "The relationship between a document and an entity documented by it."@en ;
           rdfs:isDefinedBy <https://w3id.org/sirius/ontology/hero> ;
           rdfs:label "documents"@en .


###  https://w3id.org/sirius/ontology/hero/hasObservation
:hasObservation rdf:type owl:ObjectProperty ;
                rdfs:subPropertyOf <http://www.ontologydesignpatterns.org/cp/owl/observation.owl#hasObservation> ;
                owl:inverseOf :isObservationOf ;
                rdfs:domain :AssessmentActivity ;
                rdfs:range :Observation ;
                rdfs:comment "The relationship between an assessment activity and an observation occurring during said activity."@en ;
                rdfs:isDefinedBy <https://w3id.org/sirius/ontology/hero> ;
                rdfs:label "has observation"@en .


###  https://w3id.org/sirius/ontology/hero/hasParameter
:hasParameter rdf:type owl:ObjectProperty ;
              rdfs:subPropertyOf <http://www.ontologydesignpatterns.org/cp/owl/observation.owl#hasParameter> ;
              rdfs:domain :Observation ;
              rdfs:range :Parameter ;
              rdfs:comment "A relationship between an observation happening during a contextualisation activity and a contextual parameter that is being observed as part of the context."@en ;
              rdfs:isDefinedBy <https://w3id.org/sirius/ontology/hero> ;
              rdfs:label "has parameter"@en .


###  https://w3id.org/sirius/ontology/hero/hasParticipant
:hasParticipant rdf:type owl:ObjectProperty ;
                rdfs:subPropertyOf <http://www.ontologydesignpatterns.org/cp/owl/participation.owl#hasParticipant> ;
                owl:inverseOf :isParticipantIn ;
                rdfs:domain :AssessmentActivity ;
                rdfs:range <http://xmlns.com/foaf/0.1/Agent> ;
                rdfs:comment "The relationship between an assessment activity and a participant that takes part in it."@en ;
                rdfs:isDefinedBy <https://w3id.org/sirius/ontology/hero> ;
                rdfs:label "has participant"@en .


###  https://w3id.org/sirius/ontology/hero/identifies
:identifies rdf:type owl:ObjectProperty ;
            rdfs:subPropertyOf :assesses ;
            owl:inverseOf :isIdentifiedIn ;
            rdfs:domain :IdentificationDescription ;
            rdfs:range :Risk ;
            rdfs:comment "The relationship between a identification activity and a risk that is being identified."@en ;
            rdfs:isDefinedBy <https://w3id.org/sirius/ontology/hero> ;
            rdfs:label "identifies"@en .


###  https://w3id.org/sirius/ontology/hero/isAnalysedIn
:isAnalysedIn rdf:type owl:ObjectProperty ;
              rdfs:subPropertyOf :isAssessedIn ;
              rdfs:domain :Risk ;
              rdfs:range :AnalysisDescription ;
              rdfs:comment "The relationship between a risk that is being analysed and an analysis activity."@en ;
              rdfs:isDefinedBy <https://w3id.org/sirius/ontology/hero> ;
              rdfs:label "is analysed in"@en .


###  https://w3id.org/sirius/ontology/hero/isAssessedIn
:isAssessedIn rdf:type owl:ObjectProperty ;
              rdfs:subPropertyOf <http://www.ontologydesignpatterns.org/cp/owl/timeindexedsituation.owl#hasTimeIndexedSetting> ;
              rdfs:domain :Element ;
              rdfs:range :AssessmentActivity ;
              rdfs:comment "The relationship between an entity, such as a criterion, and a assessment activity assessing it."@en ;
              rdfs:isDefinedBy <https://w3id.org/sirius/ontology/hero> ;
              rdfs:label "is assessed in"@en .


###  https://w3id.org/sirius/ontology/hero/isAssignedIn
:isAssignedIn rdf:type owl:ObjectProperty ;
              rdfs:subPropertyOf :isAssessedIn ;
              rdfs:domain :Value ;
              rdfs:range :ValueDescription ;
              rdfs:comment "The relationship between an asset value that is being assessed and a value assessment."@en ;
              rdfs:isDefinedBy <https://w3id.org/sirius/ontology/hero> ;
              rdfs:label "is assigned in"@en .


###  https://w3id.org/sirius/ontology/hero/isClassifiedBy
:isClassifiedBy rdf:type owl:ObjectProperty ;
                rdfs:subPropertyOf <http://www.ontologydesignpatterns.org/cp/owl/classification.owl#isClassifiedBy> ;
                rdfs:domain owl:Thing ;
                rdfs:range <http://www.ontologydesignpatterns.org/cp/owl/classification.owl#Concept> ;
                rdfs:comment "A relationship between a risk and another concept that may classify it, such as an agent of deterioration, a layer, or a type."@en ;
                rdfs:isDefinedBy <https://w3id.org/sirius/ontology/hero> ;
                rdfs:label "is classified by"@en .


###  https://w3id.org/sirius/ontology/hero/isClassifiedByAgent
:isClassifiedByAgent rdf:type owl:ObjectProperty ;
                     rdfs:subPropertyOf :isClassifiedBy ;
                     rdfs:domain :Risk ;
                     rdfs:range :AgentOfDeterioration ;
                     rdfs:comment "A relationship between a risk and an agent of deterioration."@en ;
                     rdfs:isDefinedBy <https://w3id.org/sirius/ontology/hero> ;
                     rdfs:label "is classified by agent"@en .


###  https://w3id.org/sirius/ontology/hero/isClassifiedByLayer
:isClassifiedByLayer rdf:type owl:ObjectProperty ;
                     rdfs:subPropertyOf :isClassifiedBy ;
                     rdfs:domain :Risk ;
                     rdfs:range :Layer ;
                     rdfs:comment "A relationship between a risk and a layer."@en ;
                     rdfs:isDefinedBy <https://w3id.org/sirius/ontology/hero> ;
                     rdfs:label "is classified by layer"@en .


###  https://w3id.org/sirius/ontology/hero/isClassifiedByType
:isClassifiedByType rdf:type owl:ObjectProperty ;
                    rdfs:subPropertyOf :isClassifiedBy ;
                    rdfs:domain :Risk ;
                    rdfs:range :RiskType ;
                    rdfs:comment "A relationship between a risk and a type."@en ;
                    rdfs:isDefinedBy <https://w3id.org/sirius/ontology/hero> ;
                    rdfs:label "is classified by type"@en .


###  https://w3id.org/sirius/ontology/hero/isDescribedIn
:isDescribedIn rdf:type owl:ObjectProperty ;
               rdfs:subPropertyOf <http://www.ontologydesignpatterns.org/cp/owl/situation.owl#hasSetting> ;
               rdfs:domain owl:Thing ;
               rdfs:range :AssessmentActivity ;
               rdfs:comment "The relationship between the entity, such as an asset, and an assessment activity assessing it."@en ;
               rdfs:isDefinedBy <https://w3id.org/sirius/ontology/hero> ;
               rdfs:label "is described in"@en .


###  https://w3id.org/sirius/ontology/hero/isDocumentedBy
:isDocumentedBy rdf:type owl:ObjectProperty ;
                rdfs:domain owl:Thing ;
                rdfs:range <http://xmlns.com/foaf/0.1/Document> ;
                rdfs:comment "The relationship between something and a Document that documents it."@en ;
                rdfs:isDefinedBy <https://w3id.org/sirius/ontology/hero> ;
                rdfs:label "is documented by" .


###  https://w3id.org/sirius/ontology/hero/isIdentifiedIn
:isIdentifiedIn rdf:type owl:ObjectProperty ;
                rdfs:subPropertyOf :isAssessedIn ;
                rdfs:domain :Risk ;
                rdfs:range :IdentificationDescription ;
                rdfs:comment "The relationship between a risk that is being identified and a identification activity."@en ;
                rdfs:isDefinedBy <https://w3id.org/sirius/ontology/hero> ;
                rdfs:label "is identified in"@en .


###  https://w3id.org/sirius/ontology/hero/isObservationOf
:isObservationOf rdf:type owl:ObjectProperty ;
                 rdfs:subPropertyOf <http://www.ontologydesignpatterns.org/cp/owl/observation.owl#isObservationOf> ;
                 rdfs:domain :Observation ;
                 rdfs:range :AssessmentActivity ;
                 rdfs:comment "The relationship between an observation and an assessment activity."@en ;
                 rdfs:isDefinedBy <https://w3id.org/sirius/ontology/hero> ;
                 rdfs:label "is observation of"@en .


###  https://w3id.org/sirius/ontology/hero/isParticipantIn
:isParticipantIn rdf:type owl:ObjectProperty ;
                 rdfs:subPropertyOf <http://www.ontologydesignpatterns.org/cp/owl/participation.owl#isParticipantIn> ;
                 rdfs:domain <http://xmlns.com/foaf/0.1/Agent> ;
                 rdfs:range :AssessmentActivity ;
                 rdfs:comment "The relationship between an agent and an assessment activity."@en ;
                 rdfs:isDefinedBy <https://w3id.org/sirius/ontology/hero> ;
                 rdfs:label "is participant in"@en .


###  https://w3id.org/sirius/ontology/hero/isQuantifiedBy
:isQuantifiedBy rdf:type owl:ObjectProperty ;
                rdfs:subPropertyOf <http://www.ontologydesignpatterns.org/cp/owl/region.owl#isRegionFor> ;
                owl:inverseOf :quantifies ;
                rdfs:domain :Measure ;
                rdfs:range :AnalysisDescription ;
                rdfs:comment "The relationship between a measure and an analysis activity."@en ;
                rdfs:isDefinedBy <https://w3id.org/sirius/ontology/hero> ;
                rdfs:label "is quantified by"@en .


###  https://w3id.org/sirius/ontology/hero/quantifies
:quantifies rdf:type owl:ObjectProperty ;
            rdfs:subPropertyOf <http://www.ontologydesignpatterns.org/cp/owl/region.owl#hasRegion> ;
            rdfs:domain :AnalysisDescription ;
            rdfs:range :Measure ;
            rdfs:comment "The relationship between an analysis activity and a measure considered during the analysis."@en ;
            rdfs:isDefinedBy <https://w3id.org/sirius/ontology/hero> ;
            rdfs:label "quantifies"@en .


#################################################################
#    Data properties
#################################################################

###  http://www.ontologydesignpatterns.org/cp/owl/observation.owl#inDate
<http://www.ontologydesignpatterns.org/cp/owl/observation.owl#inDate> rdf:type owl:DatatypeProperty ;
                                                                      rdfs:domain <http://www.ontologydesignpatterns.org/cp/owl/observation.owl#Observation> ;
                                                                      rdfs:comment "A property that assigns a datetime to a Observation."@en ;
                                                                      rdfs:isDefinedBy <http://www.ontologydesignpatterns.org/cp/owl/observation.owl> ;
                                                                      rdfs:label "in date"@en .


###  http://www.ontologydesignpatterns.org/cp/owl/region.owl#hasRegionDataValue
<http://www.ontologydesignpatterns.org/cp/owl/region.owl#hasRegionDataValue> rdf:type owl:DatatypeProperty ;
                                                                             rdfs:domain <http://www.ontologydesignpatterns.org/cp/owl/region.owl#Region> ;
                                                                             rdfs:comment "A datatype property that encodes values for a Region, e.g. a float for the Region Height." ;
                                                                             rdfs:isDefinedBy <http://www.ontologydesignpatterns.org/cp/owl/region.owl> ;
                                                                             rdfs:label "has region data value"@en ,
                                                                                        "regione ha valore {it}" .


###  http://www.ontologydesignpatterns.org/cp/owl/timeinterval.owl#hasIntervalDate
<http://www.ontologydesignpatterns.org/cp/owl/timeinterval.owl#hasIntervalDate> rdf:type owl:DatatypeProperty ;
                                                                                rdfs:domain <http://www.ontologydesignpatterns.org/cp/owl/timeinterval.owl#TimeInterval> ;
                                                                                rdfs:comment "A datatype property that encodes values from xsd:date (or any other date-related xsd datatype) for a TimeInterval; a same TimeInterval can have more than one date value: begin date, end date, date at which the interval holds, as well as dates expressed in different formats: xsd:gYear, xsd:dateTime, etc." ;
                                                                                rdfs:isDefinedBy <http://www.ontologydesignpatterns.org/cp/owl/timeinterval.owl> ;
                                                                                rdfs:label "has interval date"@en ,
                                                                                           "intervallo ha data"@it .


###  http://www.ontologydesignpatterns.org/cp/owl/timeinterval.owl#hasIntervalEndDate
<http://www.ontologydesignpatterns.org/cp/owl/timeinterval.owl#hasIntervalEndDate> rdf:type owl:DatatypeProperty ;
                                                                                   rdfs:subPropertyOf <http://www.ontologydesignpatterns.org/cp/owl/timeinterval.owl#hasIntervalDate> ;
                                                                                   rdfs:domain <http://www.ontologydesignpatterns.org/cp/owl/timeinterval.owl#TimeInterval> ;
                                                                                   rdfs:comment "The end date of a time interval." ;
                                                                                   rdfs:isDefinedBy <http://www.ontologydesignpatterns.org/cp/owl/timeinterval.owl> ;
                                                                                   rdfs:label "interval has end date"@en .


###  http://www.ontologydesignpatterns.org/cp/owl/timeinterval.owl#hasIntervalStartDate
<http://www.ontologydesignpatterns.org/cp/owl/timeinterval.owl#hasIntervalStartDate> rdf:type owl:DatatypeProperty ;
                                                                                     rdfs:subPropertyOf <http://www.ontologydesignpatterns.org/cp/owl/timeinterval.owl#hasIntervalDate> ;
                                                                                     rdfs:domain <http://www.ontologydesignpatterns.org/cp/owl/timeinterval.owl#TimeInterval> ;
                                                                                     rdfs:comment "The start date of a time interval." ;
                                                                                     rdfs:isDefinedBy <http://www.ontologydesignpatterns.org/cp/owl/timeinterval.owl> ;
                                                                                     rdfs:label "interval has start date"@en .


###  https://w3id.org/sirius/ontology/hero/assessesPercentage
:assessesPercentage rdf:type owl:DatatypeProperty ;
                    rdfs:domain :ValueDescription ;
                    rdfs:range xsd:integer ;
                    rdfs:comment "A property that assigns a value percentage to an asset which has been assigned a value in a value description."@en ;
                    rdfs:isDefinedBy <https://w3id.org/sirius/ontology/hero> ;
                    rdfs:label "assessesPercentage"@en .


###  https://w3id.org/sirius/ontology/hero/hasEstimate
:hasEstimate rdf:type owl:DatatypeProperty ;
             rdfs:subPropertyOf <http://www.ontologydesignpatterns.org/cp/owl/region.owl#hasRegionDataValue> ;
             rdfs:domain :Measure ;
             rdfs:range xsd:decimal ;
             rdfs:comment "A property that assigns a estimate value to a measure."@en ;
             rdfs:isDefinedBy <https://w3id.org/sirius/ontology/hero> ;
             rdfs:label "has estimate"@en .


###  https://w3id.org/sirius/ontology/hero/hasHighEstimate
:hasHighEstimate rdf:type owl:DatatypeProperty ;
                 rdfs:subPropertyOf :hasEstimate ;
                 rdfs:domain :Measure ;
                 rdfs:range xsd:decimal ;
                 rdfs:comment "A property that assigns a estimate value for the worst case scenario to a measure."@en ;
                 rdfs:isDefinedBy <https://w3id.org/sirius/ontology/hero> ;
                 rdfs:label "has high estimate" .


###  https://w3id.org/sirius/ontology/hero/hasLowEstimate
:hasLowEstimate rdf:type owl:DatatypeProperty ;
                rdfs:subPropertyOf :hasEstimate ;
                rdfs:domain :Measure ;
                rdfs:range xsd:decimal ;
                rdfs:comment "A property that assigns a estimate value for the best case scenario to a measure."@en ;
                rdfs:isDefinedBy <https://w3id.org/sirius/ontology/hero> ;
                rdfs:label "has low estimate" .


###  https://w3id.org/sirius/ontology/hero/hasNote
:hasNote rdf:type owl:DatatypeProperty ;
         rdfs:domain owl:Thing ;
         rdfs:range rdfs:Literal ;
         rdfs:comment "A property that assigns a textual description to something."@en ;
         rdfs:isDefinedBy <https://w3id.org/sirius/ontology/hero> ;
         rdfs:label "has note"@en .


###  https://w3id.org/sirius/ontology/hero/hasProbableEstimate
:hasProbableEstimate rdf:type owl:DatatypeProperty ;
                     rdfs:subPropertyOf :hasEstimate ;
                     rdfs:domain :Measure ;
                     rdfs:range xsd:decimal ;
                     rdfs:comment "A property that assigns a estimate value for the most likely case scenario to a measure."@en ;
                     rdfs:isDefinedBy <https://w3id.org/sirius/ontology/hero> ;
                     rdfs:label "has probable estimate" .


###  https://w3id.org/sirius/ontology/hero/hasScore
:hasScore rdf:type owl:DatatypeProperty ;
          rdfs:subPropertyOf <http://www.ontologydesignpatterns.org/cp/owl/region.owl#hasRegionDataValue> ;
          rdfs:domain :Value ;
          rdfs:range xsd:integer ;
          rdfs:comment "A property that assigns a numerical estimate to quantify an asset value."@en ;
          rdfs:isDefinedBy <https://w3id.org/sirius/ontology/hero> ;
          rdfs:label "has score"@en .


###  https://w3id.org/sirius/ontology/hero/inDate
:inDate rdf:type owl:DatatypeProperty ;
        rdfs:subPropertyOf <http://www.ontologydesignpatterns.org/cp/owl/observation.owl#inDate> ;
        rdfs:domain :Observation ;
        rdfs:range xsd:dateTime ;
        rdfs:comment "A property that assigns a datetime value to an observation."@en ;
        rdfs:isDefinedBy <https://w3id.org/sirius/ontology/hero> ;
        rdfs:label "in date"@en .


#################################################################
#    Classes
#################################################################

###  http://www.ontologydesignpatterns.org/cp/owl/classification.owl#Concept
<http://www.ontologydesignpatterns.org/cp/owl/classification.owl#Concept> rdf:type owl:Class ;
                                                                          rdfs:comment """A concept is a Social Object. 
The classifies relation relates concepts to entities at some time, but time can only be expressed in the alternative pattern: timeindexedclassification.""" ;
                                                                          rdfs:isDefinedBy <http://www.ontologydesignpatterns.org/cp/owl/classification.owl> ;
                                                                          rdfs:label "Concept"@en ,
                                                                                     "Concetto"@it .


###  http://www.ontologydesignpatterns.org/cp/owl/observation.owl#Observation
<http://www.ontologydesignpatterns.org/cp/owl/observation.owl#Observation> rdf:type owl:Class ;
                                                                           rdfs:subClassOf <http://www.ontologydesignpatterns.org/cp/owl/situation.owl#Situation> ,
                                                                                           [ rdf:type owl:Restriction ;
                                                                                             owl:onProperty <http://www.ontologydesignpatterns.org/cp/owl/observation.owl#hasParameter> ;
                                                                                             owl:someValuesFrom <http://www.ontologydesignpatterns.org/cp/owl/observation.owl#Parameter>
                                                                                           ] ,
                                                                                           [ rdf:type owl:Restriction ;
                                                                                             owl:onProperty <http://www.ontologydesignpatterns.org/cp/owl/observation.owl#isObservationOf> ;
                                                                                             owl:someValuesFrom owl:Thing
                                                                                           ] ,
                                                                                           [ rdf:type owl:Restriction ;
                                                                                             owl:onProperty <http://www.ontologydesignpatterns.org/cp/owl/observation.owl#inDate> ;
                                                                                             owl:cardinality "1"^^xsd:nonNegativeInteger
                                                                                           ] ;
                                                                           rdfs:comment "A specific situation where some thing is observed with respect ot a set of parameters." ;
                                                                           rdfs:isDefinedBy <http://www.ontologydesignpatterns.org/cp/owl/observation.owl> ;
                                                                           rdfs:label "Observation"@en .


###  http://www.ontologydesignpatterns.org/cp/owl/observation.owl#Parameter
<http://www.ontologydesignpatterns.org/cp/owl/observation.owl#Parameter> rdf:type owl:Class ;
                                                                         rdfs:subClassOf <http://www.ontologydesignpatterns.org/cp/owl/region.owl#Region> ;
                                                                         owl:disjointWith <http://www.ontologydesignpatterns.org/cp/owl/situation.owl#Situation> ;
                                                                         rdfs:comment "The parameters of an observation describe the context and content of the observation. For example in a medical context an observation of a patient may contain a set of symptoms, that are the parameters of that observation." ;
                                                                         rdfs:isDefinedBy <http://www.ontologydesignpatterns.org/cp/owl/observation.owl> ;
                                                                         rdfs:label "Parameter"@en .


###  http://www.ontologydesignpatterns.org/cp/owl/participation.owl#Event
<http://www.ontologydesignpatterns.org/cp/owl/participation.owl#Event> rdf:type owl:Class ;
                                                                       rdfs:subClassOf [ rdf:type owl:Restriction ;
                                                                                         owl:onProperty <http://www.ontologydesignpatterns.org/cp/owl/participation.owl#hasParticipant> ;
                                                                                         owl:someValuesFrom <http://www.ontologydesignpatterns.org/cp/owl/participation.owl#Object>
                                                                                       ] ;
                                                                       owl:disjointWith <http://www.ontologydesignpatterns.org/cp/owl/participation.owl#Object> ;
                                                                       rdfs:comment "Any physical, social, or mental process, event, or state." ;
                                                                       rdfs:isDefinedBy <http://www.ontologydesignpatterns.org/cp/owl/participation.owl> ;
                                                                       rdfs:label "Event"@en .


###  http://www.ontologydesignpatterns.org/cp/owl/participation.owl#Object
<http://www.ontologydesignpatterns.org/cp/owl/participation.owl#Object> rdf:type owl:Class ;
                                                                        rdfs:subClassOf [ rdf:type owl:Restriction ;
                                                                                          owl:onProperty <http://www.ontologydesignpatterns.org/cp/owl/participation.owl#isParticipantIn> ;
                                                                                          owl:someValuesFrom <http://www.ontologydesignpatterns.org/cp/owl/participation.owl#Event>
                                                                                        ] ;
                                                                        rdfs:comment "Any physical, social, or mental object, or substance" ;
                                                                        rdfs:isDefinedBy <http://www.ontologydesignpatterns.org/cp/owl/participation.owl> ;
                                                                        rdfs:label "Object"@en .


###  http://www.ontologydesignpatterns.org/cp/owl/region.owl#Region
<http://www.ontologydesignpatterns.org/cp/owl/region.owl#Region> rdf:type owl:Class ;
                                                                 rdfs:subClassOf [ rdf:type owl:Restriction ;
                                                                                   owl:onProperty <http://www.ontologydesignpatterns.org/cp/owl/region.owl#isRegionFor> ;
                                                                                   owl:allValuesFrom owl:Thing
                                                                                 ] ;
                                                                 rdfs:comment """Any region in a dimensional space (a dimensional space is a maximal Region), which can be used as a value for a quality of an Entity . For example, TimeInterval, SpaceRegion, PhysicalAttribute, Amount, SocialAttribute are all subclasses of Region. 
Regions are not data values in the ordinary knowledge representation sense; in order to get patterns for modelling data, see the properties: representsDataValue and hasDataValue""" ;
                                                                 rdfs:isDefinedBy <http://www.ontologydesignpatterns.org/cp/owl/region.owl> ;
                                                                 rdfs:label "Region"@en ,
                                                                            "Regione"@it .


###  http://www.ontologydesignpatterns.org/cp/owl/situation.owl#Situation
<http://www.ontologydesignpatterns.org/cp/owl/situation.owl#Situation> rdf:type owl:Class .


###  http://www.ontologydesignpatterns.org/cp/owl/timeindexedsituation.owl#TimeIndexedSituation
<http://www.ontologydesignpatterns.org/cp/owl/timeindexedsituation.owl#TimeIndexedSituation> rdf:type owl:Class ;
                                                                                             rdfs:subClassOf <http://www.ontologydesignpatterns.org/cp/owl/situation.owl#Situation> ,
                                                                                                             [ rdf:type owl:Restriction ;
                                                                                                               owl:onProperty <http://www.ontologydesignpatterns.org/cp/owl/timeindexedsituation.owl#atTime> ;
                                                                                                               owl:minCardinality "1"^^xsd:nonNegativeInteger
                                                                                                             ] ,
                                                                                                             [ rdf:type owl:Restriction ;
                                                                                                               owl:onProperty <http://www.ontologydesignpatterns.org/cp/owl/timeindexedsituation.owl#forEntity> ;
                                                                                                               owl:minCardinality "1"^^xsd:nonNegativeInteger
                                                                                                             ] ;
                                                                                             rdfs:comment "A Situation that is explicitly indexed at some time for at least one entity." ;
                                                                                             rdfs:isDefinedBy <http://www.ontologydesignpatterns.org/cp/owl/timeindexedsituation.owl> ;
                                                                                             rdfs:label "Time indexed situation"@en .


###  http://www.ontologydesignpatterns.org/cp/owl/timeinterval.owl#TimeInterval
<http://www.ontologydesignpatterns.org/cp/owl/timeinterval.owl#TimeInterval> rdf:type owl:Class ;
                                                                             rdfs:subClassOf <http://www.ontologydesignpatterns.org/cp/owl/region.owl#Region> ,
                                                                                             [ rdf:type owl:Restriction ;
                                                                                               owl:onProperty <http://www.ontologydesignpatterns.org/cp/owl/timeinterval.owl#hasIntervalEndDate> ;
                                                                                               owl:maxCardinality "1"^^xsd:nonNegativeInteger
                                                                                             ] ,
                                                                                             [ rdf:type owl:Restriction ;
                                                                                               owl:onProperty <http://www.ontologydesignpatterns.org/cp/owl/timeinterval.owl#hasIntervalStartDate> ;
                                                                                               owl:maxCardinality "1"^^xsd:nonNegativeInteger
                                                                                             ] ;
                                                                             rdfs:comment """Any Region in a dimensional space that aims at representing time.
It should be used when you want to talk about time as an object having some characteristics.""" ;
                                                                             rdfs:isDefinedBy <http://www.ontologydesignpatterns.org/cp/owl/timeinterval.owl> ;
                                                                             rdfs:label "Intervallo di tempo"@it ,
                                                                                        "Time interval"@en .


###  http://www.w3.org/2002/07/owl#Thing
owl:Thing rdf:type owl:Class .


###  http://xmlns.com/foaf/0.1/Agent
<http://xmlns.com/foaf/0.1/Agent> rdf:type owl:Class ;
                                  rdfs:comment "An agent (eg. person, group, software or physical artifact)."@en ;
                                  rdfs:label "Agent"@en .


###  http://xmlns.com/foaf/0.1/Document
<http://xmlns.com/foaf/0.1/Document> rdf:type owl:Class ;
                                     rdfs:comment "A document."@en ;
                                     rdfs:label "Document"@en .


###  https://w3id.org/sirius/ontology/hero/AgentOfDeterioration
:AgentOfDeterioration rdf:type owl:Class ;
                      rdfs:subClassOf <http://www.ontologydesignpatterns.org/cp/owl/classification.owl#Concept> ;
                      rdfs:comment "A conceptualization used to classify a risk threatening an asset, made from the perspective of the asset itself."@en ;
                      rdfs:isDefinedBy <https://w3id.org/sirius/ontology/hero> ;
                      rdfs:label "Agent of deterioration"@en .


###  https://w3id.org/sirius/ontology/hero/AnalysisDescription
:AnalysisDescription rdf:type owl:Class ;
                     rdfs:subClassOf :AssessmentActivity ;
                     rdfs:comment "An activity that involves the quantification of risks to understand their magnitude and potential impact with respect to an asset."@en ;
                     rdfs:isDefinedBy <https://w3id.org/sirius/ontology/hero> ;
                     rdfs:label "Analysis description"@en .


###  https://w3id.org/sirius/ontology/hero/Aspect
:Aspect rdf:type owl:Class ;
        rdfs:subClassOf <http://www.ontologydesignpatterns.org/cp/owl/classification.owl#Concept> ;
        rdfs:comment "A facet of the context that contributes to the overall understanding and assessment of the asset value."@en ;
        rdfs:isDefinedBy <https://w3id.org/sirius/ontology/hero> ;
        rdfs:label "Aspect"@en .


###  https://w3id.org/sirius/ontology/hero/AssessmentActivity
:AssessmentActivity rdf:type owl:Class ;
                    rdfs:subClassOf <http://www.ontologydesignpatterns.org/cp/owl/participation.owl#Event> ,
                                    <http://www.ontologydesignpatterns.org/cp/owl/timeindexedsituation.owl#TimeIndexedSituation> ;
                    rdfs:comment "A situation consisting in the assessment of the risks related to an asset."@en ;
                    rdfs:isDefinedBy <https://w3id.org/sirius/ontology/hero> ;
                    rdfs:label "Assessment activity"@en .


###  https://w3id.org/sirius/ontology/hero/ContextDescription
:ContextDescription rdf:type owl:Class ;
                    rdfs:subClassOf :AssessmentActivity ;
                    rdfs:comment "An activity that involves the examination of the contextual information of an asset."@en ;
                    rdfs:isDefinedBy <https://w3id.org/sirius/ontology/hero> ;
                    rdfs:label "Context description"@en .


###  https://w3id.org/sirius/ontology/hero/Dimension
:Dimension rdf:type owl:Class ;
           rdfs:subClassOf <http://www.ontologydesignpatterns.org/cp/owl/classification.owl#Concept> ;
           rdfs:comment "A facet of an asset that contributes to the overall understanding and assessment of its value."@en ;
           rdfs:isDefinedBy <https://w3id.org/sirius/ontology/hero> ;
           rdfs:label "Dimension"@en .


###  https://w3id.org/sirius/ontology/hero/Element
:Element rdf:type owl:Class ;
         rdfs:subClassOf <http://www.ontologydesignpatterns.org/cp/owl/region.owl#Region> ;
         rdfs:comment "A conceptual category used as a basis for evaluating an asset during a risk assessment activity."@en ;
         rdfs:isDefinedBy <https://w3id.org/sirius/ontology/hero> ;
         rdfs:label "Element"@en .


###  https://w3id.org/sirius/ontology/hero/Exposure
:Exposure rdf:type owl:Class ;
          rdfs:subClassOf :Measure ;
          rdfs:comment "The size of the expected loss of value in the whole asset affected by the risk."@en ;
          rdfs:isDefinedBy <https://w3id.org/sirius/ontology/hero> ;
          rdfs:label "Exposure"@en .


###  https://w3id.org/sirius/ontology/hero/FractionalValueLoss
:FractionalValueLoss rdf:type owl:Class ;
                     rdfs:subClassOf :Measure ;
                     rdfs:comment "The size of the expected loss of value in each part of the asset affected by the risk."@en ;
                     rdfs:isDefinedBy <https://w3id.org/sirius/ontology/hero> ;
                     rdfs:label "Fractional value loss" .


###  https://w3id.org/sirius/ontology/hero/Frequency
:Frequency rdf:type owl:Class ;
           rdfs:subClassOf :Measure ;
           rdfs:comment "The likelihood or probability of a specific risk event occurring within a given period. It quantifies how often a particular risk is expected to materialize and helps assess the regularity or recurrence of the risk."@en ;
           rdfs:isDefinedBy <https://w3id.org/sirius/ontology/hero> ;
           rdfs:label "Frequency" .


###  https://w3id.org/sirius/ontology/hero/IdentificationDescription
:IdentificationDescription rdf:type owl:Class ;
                           rdfs:subClassOf :AssessmentActivity ;
                           rdfs:comment "An activity that involves the identification of risks to understand their nature, causes, and consequences with respect to an asset."@en ;
                           rdfs:isDefinedBy <https://w3id.org/sirius/ontology/hero> ;
                           rdfs:label "Identification description"@en .


###  https://w3id.org/sirius/ontology/hero/Layer
:Layer rdf:type owl:Class ;
       rdfs:subClassOf <http://www.ontologydesignpatterns.org/cp/owl/classification.owl#Concept> ;
       rdfs:comment "A conceptualization used to classify a risk threatening an asset on the basis of the spatial context in which the asset exists."@en ;
       rdfs:isDefinedBy <https://w3id.org/sirius/ontology/hero> ;
       rdfs:label "Layer"@en .


###  https://w3id.org/sirius/ontology/hero/Magnitude
:Magnitude rdf:type owl:Class ;
           rdfs:subClassOf :Measure ;
           rdfs:comment "The quantified extension of a risk, encompassing the overall impact and severity associated with it if it were to occur."@en ;
           rdfs:isDefinedBy <https://w3id.org/sirius/ontology/hero> ;
           rdfs:label "Magnitude"@en .


###  https://w3id.org/sirius/ontology/hero/Measure
:Measure rdf:type owl:Class ;
         owl:equivalentClass [ owl:intersectionOf ( <http://www.ontologydesignpatterns.org/cp/owl/region.owl#Region>
                                                    [ rdf:type owl:Restriction ;
                                                      owl:onProperty :hasEstimate ;
                                                      owl:someValuesFrom xsd:decimal
                                                    ]
                                                  ) ;
                               rdf:type owl:Class
                             ] ;
         rdfs:subClassOf <http://www.ontologydesignpatterns.org/cp/owl/region.owl#Region> ;
         rdfs:comment "A quantifiable aspect of some entity, that expresses a more precise and standardised evaluation of it, based on assigning numerical values or metrics to some specific attributes."@en ;
         rdfs:isDefinedBy <https://w3id.org/sirius/ontology/hero> ;
         rdfs:label "Measure"@en .


###  https://w3id.org/sirius/ontology/hero/Observation
:Observation rdf:type owl:Class ;
             rdfs:subClassOf <http://www.ontologydesignpatterns.org/cp/owl/observation.owl#Observation> ;
             rdfs:comment "An observation about an asset during an assessment activity."@en ;
             rdfs:isDefinedBy <https://w3id.org/sirius/ontology/hero> ;
             rdfs:label "Observation"@en .


###  https://w3id.org/sirius/ontology/hero/Parameter
:Parameter rdf:type owl:Class ;
           rdfs:subClassOf <http://www.ontologydesignpatterns.org/cp/owl/observation.owl#Parameter> ;
           rdfs:comment "A contextual parameter used in an observation about an asset during an assessment activity."@en ;
           rdfs:isDefinedBy <https://w3id.org/sirius/ontology/hero> ;
           rdfs:label "Parameter"@en .


###  https://w3id.org/sirius/ontology/hero/Risk
:Risk rdf:type owl:Class ;
      rdfs:subClassOf :Element ;
      rdfs:comment "The possibility of a loss of value to an asset."@en ;
      rdfs:isDefinedBy <https://w3id.org/sirius/ontology/hero> ;
      rdfs:label "Risk"@en .


###  https://w3id.org/sirius/ontology/hero/RiskType
:RiskType rdf:type owl:Class ;
          rdfs:subClassOf <http://www.ontologydesignpatterns.org/cp/owl/classification.owl#Concept> ;
          rdfs:comment "A conceptualization used to classify a risk according to its type of occurrence."@en ;
          rdfs:isDefinedBy <https://w3id.org/sirius/ontology/hero> ;
          rdfs:label "Risk type"@en .


###  https://w3id.org/sirius/ontology/hero/Value
:Value rdf:type owl:Class ;
       rdfs:subClassOf :Element ;
       rdfs:comment "A quality that represents the perceived significance or importance assigned to an asset."@en ;
       rdfs:isDefinedBy <https://w3id.org/sirius/ontology/hero> ;
       rdfs:label "Value"@en .


###  https://w3id.org/sirius/ontology/hero/ValueDescription
:ValueDescription rdf:type owl:Class ;
                  rdfs:subClassOf :AssessmentActivity ;
                  rdfs:comment "An activity that involves the identification of values that contribute to the perceived importance of an asset."@en ;
                  rdfs:isDefinedBy <https://w3id.org/sirius/ontology/hero> ;
                  rdfs:label "Value description"@en .


#################################################################
#    Individuals
#################################################################

###  https://w3id.org/sirius/ontology/hero/administrative
:administrative rdf:type owl:NamedIndividual ,
                         :Parameter ;
                rdfs:comment "A contextual parameter representing the administrative environment of the heritage asset."@en ;
                rdfs:isDefinedBy <https://w3id.org/sirius/ontology/hero> ;
                rdfs:label "Administrative"@en .


###  https://w3id.org/sirius/ontology/hero/artistic
:artistic rdf:type owl:NamedIndividual ,
                   :Dimension ;
          rdfs:comment "The dimension referring to the aesthetic qualities associated with an asset."@en ;
          rdfs:isDefinedBy <https://w3id.org/sirius/ontology/hero> ;
          rdfs:label "Artistic"@en .


###  https://w3id.org/sirius/ontology/hero/building
:building rdf:type owl:NamedIndividual ,
                   :Layer ;
          rdfs:comment "A layer that encapsulates the entire building that houses the heritage asset."@en ;
          rdfs:isDefinedBy <https://w3id.org/sirius/ontology/hero> ;
          rdfs:label "Building"@en .


###  https://w3id.org/sirius/ontology/hero/common
:common rdf:type owl:NamedIndividual ,
                 :RiskType ;
        rdfs:comment "A type of risk that occurs many times per century."@en ;
        rdfs:isDefinedBy <https://w3id.org/sirius/ontology/hero> ;
        rdfs:label "Common"@en .


###  https://w3id.org/sirius/ontology/hero/cumulative
:cumulative rdf:type owl:NamedIndividual ,
                     :RiskType ;
            rdfs:comment "A type of risk that can occur continuously or intermittently."@en ;
            rdfs:isDefinedBy <https://w3id.org/sirius/ontology/hero> ;
            rdfs:label "Cumulative"@en .


###  https://w3id.org/sirius/ontology/hero/dissociation
:dissociation rdf:type owl:NamedIndividual ,
                       :AgentOfDeterioration ;
              rdfs:comment "An agent of deterioration that includes the natural tendency for ordered systems to fall apart over time."@en ;
              rdfs:isDefinedBy <https://w3id.org/sirius/ontology/hero> ;
              rdfs:label "Dissociation"@en .


###  https://w3id.org/sirius/ontology/hero/economic
:economic rdf:type owl:NamedIndividual ,
                   :Parameter ;
          rdfs:comment "A contextual parameter representing the economic environment of the heritage asset."@en ;
          rdfs:isDefinedBy <https://w3id.org/sirius/ontology/hero> ;
          rdfs:label "Economic"@en .


###  https://w3id.org/sirius/ontology/hero/feeling
:feeling rdf:type owl:NamedIndividual ,
                  :Aspect ;
         rdfs:comment "An aspect that encompasses the intangible and emotional aspects associated with an asset."@en ;
         rdfs:isDefinedBy <https://w3id.org/sirius/ontology/hero> ;
         rdfs:label "Feeling"@en .


###  https://w3id.org/sirius/ontology/hero/fire
:fire rdf:type owl:NamedIndividual ,
               :AgentOfDeterioration ;
      rdfs:comment "An agent of deterioration representing the destruction of an asset due to properties of fire, such as heat, flames, or smoke."@en ;
      rdfs:isDefinedBy <https://w3id.org/sirius/ontology/hero> ;
      rdfs:label "Fire"@en .


###  https://w3id.org/sirius/ontology/hero/fitting
:fitting rdf:type owl:NamedIndividual ,
                  :Layer ;
         rdfs:comment "A layer that encapsulate the first, closest movable space to the asset."@en ;
         rdfs:isDefinedBy <https://w3id.org/sirius/ontology/hero> ;
         rdfs:label "Fitting"@en .


###  https://w3id.org/sirius/ontology/hero/form
:form rdf:type owl:NamedIndividual ,
               :Aspect ;
      rdfs:comment "An aspect that refers to the physical characteristics and appearance of an asset."@en ;
      rdfs:isDefinedBy <https://w3id.org/sirius/ontology/hero> ;
      rdfs:label "Form"@en .


###  https://w3id.org/sirius/ontology/hero/function
:function rdf:type owl:NamedIndividual ,
                   :Aspect ;
          rdfs:comment "An aspect that pertains to the purpose and use of an asset."@en ;
          rdfs:isDefinedBy <https://w3id.org/sirius/ontology/hero> ;
          rdfs:label "Function"@en .


###  https://w3id.org/sirius/ontology/hero/historic
:historic rdf:type owl:NamedIndividual ,
                   :Dimension ;
          rdfs:comment "A dimension that refers to the historical context, significance, and evolution of an asset"@en ;
          rdfs:isDefinedBy <https://w3id.org/sirius/ontology/hero> ;
          rdfs:label "Historic"@en .


###  https://w3id.org/sirius/ontology/hero/incorrect-relative-humidity
:incorrect-relative-humidity rdf:type owl:NamedIndividual ,
                                      :AgentOfDeterioration ;
                             rdfs:comment "An agent of deterioration representing the situation in which the level of humidity in the environment deviates from the optimal or specified range."@en ;
                             rdfs:isDefinedBy <https://w3id.org/sirius/ontology/hero> ;
                             rdfs:label "Incorrect relative humidity"@en .


###  https://w3id.org/sirius/ontology/hero/incorrect-temperature
:incorrect-temperature rdf:type owl:NamedIndividual ,
                                :AgentOfDeterioration ;
                       rdfs:comment "An agent of deterioration representing a situation in which the ambient temperature deviates from the optimal or specified range."@en ;
                       rdfs:isDefinedBy <https://w3id.org/sirius/ontology/hero> ;
                       rdfs:label "Incorrect temperature"@en .


###  https://w3id.org/sirius/ontology/hero/legal
:legal rdf:type owl:NamedIndividual ,
                :Parameter ;
       rdfs:comment "A contextual parameter representing the legal environment of the heritage asset."@en ;
       rdfs:isDefinedBy <https://w3id.org/sirius/ontology/hero> ;
       rdfs:label "Legal"@en .


###  https://w3id.org/sirius/ontology/hero/light-ultraviolet-infrared
:light-ultraviolet-infrared rdf:type owl:NamedIndividual ,
                                     :AgentOfDeterioration ;
                            rdfs:comment "An agent of deterioration representing different forms of electromagnetic radiation."@en ;
                            rdfs:isDefinedBy <https://w3id.org/sirius/ontology/hero> ;
                            rdfs:label "Light, ultraviolet and infrared"@en .


###  https://w3id.org/sirius/ontology/hero/pests
:pests rdf:type owl:NamedIndividual ,
                :AgentOfDeterioration ;
       rdfs:comment "An agent of deterioration representing the presence of biological agents, such as insects, rodents, and microorganisms."@en ;
       rdfs:isDefinedBy <https://w3id.org/sirius/ontology/hero> ;
       rdfs:label "Pests"@en .


###  https://w3id.org/sirius/ontology/hero/physical
:physical rdf:type owl:NamedIndividual ,
                   :Parameter ;
          rdfs:comment "A contextual parameter representing the physical environment of the heritage asset."@en ;
          rdfs:isDefinedBy <https://w3id.org/sirius/ontology/hero> ;
          rdfs:label "Physical"@en .


###  https://w3id.org/sirius/ontology/hero/physical-forces
:physical-forces rdf:type owl:NamedIndividual ,
                          :AgentOfDeterioration ;
                 rdfs:comment "An agent of deterioration representing mechanical damage resulting from handling, transport, and vibration."@en ;
                 rdfs:isDefinedBy <https://w3id.org/sirius/ontology/hero> ;
                 rdfs:label "Physical forces"@en .


###  https://w3id.org/sirius/ontology/hero/political
:political rdf:type owl:NamedIndividual ,
                    :Parameter ;
           rdfs:comment "A contextual parameter representing the political environment of the heritage asset."@en ;
           rdfs:isDefinedBy <https://w3id.org/sirius/ontology/hero> ;
           rdfs:label "Political"@en .


###  https://w3id.org/sirius/ontology/hero/pollutants
:pollutants rdf:type owl:NamedIndividual ,
                     :AgentOfDeterioration ;
            rdfs:comment "An agent of deterioration representing the presence of substances or contaminants introduced into the environment."@en ;
            rdfs:isDefinedBy <https://w3id.org/sirius/ontology/hero> ;
            rdfs:label "Pollutants"@en .


###  https://w3id.org/sirius/ontology/hero/rare
:rare rdf:type owl:NamedIndividual ,
               :RiskType ;
      rdfs:comment "A type of risk that occurs less often than approximately once every 100 years."@en ;
      rdfs:isDefinedBy <https://w3id.org/sirius/ontology/hero> ;
      rdfs:label "Rare"@en .


###  https://w3id.org/sirius/ontology/hero/region
:region rdf:type owl:NamedIndividual ,
                 :Layer ;
        rdfs:comment "A layer that encapsulates the broadest space in which the heritage asset is considered."@en ;
        rdfs:isDefinedBy <https://w3id.org/sirius/ontology/hero> ;
        rdfs:label "Region"@en .


###  https://w3id.org/sirius/ontology/hero/room
:room rdf:type owl:NamedIndividual ,
               :Layer ;
      rdfs:comment "A layer that encapsulates the interior space where the heritage asset is located."@en ;
      rdfs:isDefinedBy <https://w3id.org/sirius/ontology/hero> ;
      rdfs:label "Room"@en .


###  https://w3id.org/sirius/ontology/hero/scientific
:scientific rdf:type owl:NamedIndividual ,
                     :Dimension ;
            rdfs:comment "A dimension that involves the application of research, documentation, and analysis techniques to understand, preserve, and interpret an asset."@en ;
            rdfs:isDefinedBy <https://w3id.org/sirius/ontology/hero> ;
            rdfs:label "Scientific"@en .


###  https://w3id.org/sirius/ontology/hero/setting
:setting rdf:type owl:NamedIndividual ,
                  :Aspect ;
         rdfs:isDefinedBy <https://w3id.org/sirius/ontology/hero> ;
         rdfs:label "Setting"@en ,
                    "The surroundings and environment in which an asset is located."@en .


###  https://w3id.org/sirius/ontology/hero/site
:site rdf:type owl:NamedIndividual ,
               :Layer ;
      rdfs:comment "A layer that encapsulates the broader area or property on which the heritage asset is situated."@en ;
      rdfs:isDefinedBy <https://w3id.org/sirius/ontology/hero> ;
      rdfs:label "Site"@en .


###  https://w3id.org/sirius/ontology/hero/social
:social rdf:type owl:NamedIndividual ,
                 :Dimension ;
        rdfs:comment "A dimension that considers the cultural and social context of an asset, including its role in shaping identity, community values, and social practices."@en ;
        rdfs:isDefinedBy <https://w3id.org/sirius/ontology/hero> ;
        rdfs:label "Social"@en .


###  https://w3id.org/sirius/ontology/hero/socio-cultural
:socio-cultural rdf:type owl:NamedIndividual ,
                         :Parameter ;
                rdfs:comment "A contextual parameter representing the socio-cultural environment of the heritage asset."@en ;
                rdfs:isDefinedBy <https://w3id.org/sirius/ontology/hero> ;
                rdfs:label "Socio-cultural"@en .


###  https://w3id.org/sirius/ontology/hero/substance
:substance rdf:type owl:NamedIndividual ,
                    :Aspect ;
           rdfs:comment "An aspect that involves the material composition and integrity of an asset."@en ;
           rdfs:isDefinedBy <https://w3id.org/sirius/ontology/hero> ;
           rdfs:label "Substance"@en .


###  https://w3id.org/sirius/ontology/hero/support
:support rdf:type owl:NamedIndividual ,
                  :Layer ;
         rdfs:comment "The immediate surroundings or foundation upon which an asset relies."@en ;
         rdfs:isDefinedBy <https://w3id.org/sirius/ontology/hero> ;
         rdfs:label "Support"@en .


###  https://w3id.org/sirius/ontology/hero/theft-vandalism
:theft-vandalism rdf:type owl:NamedIndividual ,
                          :AgentOfDeterioration ;
                 rdfs:comment "An agent of deterioration representing deliberate acts of theft, vandalism, or destruction done by humans."@en ;
                 rdfs:isDefinedBy <https://w3id.org/sirius/ontology/hero> ;
                 rdfs:label "Theft and vandalism"@en .


###  https://w3id.org/sirius/ontology/hero/tradition
:tradition rdf:type owl:NamedIndividual ,
                    :Aspect ;
           rdfs:comment "An aspect that involves the surroundings and environment in which an asset is located."@en ;
           rdfs:isDefinedBy <https://w3id.org/sirius/ontology/hero> ;
           rdfs:label "Tradition"@en .


###  https://w3id.org/sirius/ontology/hero/water
:water rdf:type owl:NamedIndividual ,
                :AgentOfDeterioration ;
       rdfs:comment "An agent of deterioration representing the damage that can occur through leaks, flooding, or high humidity levels."@en ;
       rdfs:isDefinedBy <https://w3id.org/sirius/ontology/hero> ;
       rdfs:label "Water"@en .


#################################################################
#    Annotations
#################################################################

<http://xmlns.com/wordnet/1.6/Document> rdfs:label "Document"@en .


###  Generated by the OWL API (version 5.1.18) https://github.com/owlcs/owlapi/
